proof/src/zero-knowledge/definitions/dvnizk/DVNIZKSoundness.ec
@@ -44,7 +44,7 @@ theory Soundness.
       c <@ MP.commit(rp, x);
 
       rv <@ R.gen(rp);
-      if (valid_rand_verifier rp rv x) {
+      if (valid_rand_verifier rv x) {
         b <- !language x /\ valid_rand_prover rp x /\ prove rv x c;
       } else { b <- false; }
 
